SQIR/examples/extraction/AltShor.v
@@ -26,17 +26,16 @@ Fixpoint reverse_qubits' dim n : ucom U :=
 Definition reverse_qubits n := reverse_qubits' n (n/2)%nat.
 Definition QFT_w_reverse n := QFT n >> reverse_qubits n.
 
-Fixpoint controlled_powers_var' (f : nat -> bccom) k kmax : bccom :=
+Fixpoint controlled_powers' (f : nat -> bccom) k kmax : bccom :=
   match k with
   | O    => bcskip
   | S O  => bccont (kmax - 1) (f O)
-  | S k' => bcseq (controlled_powers_var' f k' kmax)
+  | S k' => bcseq (controlled_powers' f k' kmax)
                  (bccont (kmax - k' - 1) (f k'))
   end.
-Definition controlled_powers_var (f : nat -> bccom) k : ucom U := 
-  bc2ucom (controlled_powers_var' f k k).
+Definition controlled_powers (f : nat -> bccom) k : ucom U := 
+  bc2ucom (controlled_powers' f k k).
 
-(* TODO: move to RCIR *)
 Fixpoint map_bccom (f : nat -> nat) (bc : bccom) : bccom :=
   match bc with
   | bcskip => bcskip
@@ -46,9 +45,9 @@ Fixpoint map_bccom (f : nat -> nat) (bc : bccom) : bccom :=
   | bcseq bc1 bc2 => bcseq (map_bccom f bc1) (map_bccom f bc2)
   end.
 
-Definition QPE_var k (f : nat -> bccom) : ucom U :=
+Definition QPE k (f : nat -> bccom) : ucom U :=
   npar k U_H >>
-  controlled_powers_var (fun x => map_bccom (fun q => k + q)%nat (f x)) k >>
+  controlled_powers (fun x => map_bccom (fun q => k + q)%nat (f x)) k >>
   invert (QFT_w_reverse k).
 
 Definition modexp a x N := a ^ x mod N.
@@ -56,18 +55,55 @@ Definition modmult_circuit a ainv N n i :=
   RCIR.bcelim (ModMult.modmult_rev N (modexp a (2 ^ i) N) (modexp ainv (2 ^ i) N) n).
 Definition num_qubits n : nat := n + modmult_rev_anc n.
 
-(* requires 0 < a < N, gcd a N = 1 
-   returns a circuit + the number of qubits used *)
+(* requires 0 < a < N, gcd a N = 1 *)
 Definition shor_circuit a N := 
   let m := Nat.log2 (2 * N^2)%nat in
   let n := Nat.log2 (2 * N) in
   let ainv := modinv a N in
-  let numq := num_qubits n in
   let f i := modmult_circuit a ainv N n i in
-  (X (m + n - 1) >> QPE_var m f, (m + numq)%nat, m).
+  X (m + n - 1) >> QPE m f.
 
 
 (** Proofs **)
+
+Lemma controlled_rotations_WF : forall n, well_formed (controlled_rotations n).
+Proof.
+  destruct n.
+  constructor; auto.
+  destruct n.
+  constructor; auto.
+  induction n. 
+  constructor; auto.
+  constructor. apply IHn.
+  constructor; auto. 
+Qed.
+
+Local Transparent SQIR.Rz SQIR.CNOT.
+Lemma controlled_rotations_WT : forall n, (n > 0)%nat ->
+  uc_well_typed (to_base_ucom n (controlled_rotations n)).
+Proof.
+  intros n Hn.
+  destruct n; try lia.
+  clear Hn.
+  destruct n. constructor. lia.
+  induction n. repeat constructor; lia.
+  replace (controlled_rotations (S (S (S n)))) 
+    with (controlled_rotations (S (S n)) >> 
+          CU1 (2 * PI / 2 ^ (S (S (S n)))) (S (S n)) 0) 
+    by reflexivity.
+  remember (S (S n)) as n'.
+  replace (to_base_ucom (S n') (controlled_rotations n' >> 
+           CU1 (2 * PI / 2 ^ S n') n' 0))
+    with (to_base_ucom (S n') (controlled_rotations n') ;
+          to_base_ucom (S n') (CU1 (2 * PI / 2 ^ S n') n' 0))%ucom
+    by reflexivity.
+  constructor.
+  eapply change_dim_WT; try apply IHn.
+  lia.
+  apply controlled_rotations_WF.
+  repeat constructor; lia. 
+Qed.
+Local Opaque SQIR.Rz SQIR.CNOT.
 
 Lemma controlled_rotations_same : forall n,
   uc_eval n (controlled_rotations n) = 
@@ -93,10 +129,27 @@ Proof.
   rewrite <- (pad_dims_r (QPE.controlled_rotations _)).
   rewrite IHn.
   reflexivity.
+  apply QPE.controlled_rotations_WT.
+  lia.
   apply controlled_rotations_WT.
   lia.
-  admit. (* uc_well_typed (to_base_ucom n' (controlled_rotations n')) *) 
-Admitted.
+Qed.
+
+Local Opaque controlled_rotations.
+Lemma QFT_WF : forall n, well_formed (QFT n).
+Proof.
+  destruct n.
+  constructor; auto.
+  induction n.
+  constructor; auto.
+  simpl.
+  constructor.
+  constructor.
+  constructor; auto.
+  apply controlled_rotations_WF.
+  apply map_qubits_WF.
+  apply IHn.
+Qed.
 
 Lemma QFT_same : forall n,
   uc_eval n (QFT n) = UnitarySem.uc_eval (QPE.QFT n).
@@ -125,10 +178,10 @@ Proof.
   rewrite <- aux; clear aux. 
   rewrite <- IHn. 
   reflexivity.
-  admit. (* well_formed (QFT (S n)) *)
+  apply QFT_WF.
   rewrite <- change_dim.
   apply controlled_rotations_same.
-Admitted.
+Qed.
 
 Lemma reverse_qubits_same : forall n,
   uc_eval n (reverse_qubits n) = UnitarySem.uc_eval (QPE.reverse_qubits n).
@@ -147,6 +200,20 @@ Proof.
   apply H.
 Qed.
 
+Lemma reverse_qubits_WF : forall n, well_formed (reverse_qubits n).
+Proof.
+  assert (H : forall n dim, well_formed (reverse_qubits' dim n)).
+  { intros n dim.
+    destruct n.
+    constructor; auto.
+    induction n.
+    constructor; auto.
+    simpl. constructor. 
+    apply IHn.
+    constructor; auto. }
+  intro. apply H.
+Qed.
+
 Lemma QFT_w_reverse_same : forall n,
   uc_eval n (QFT_w_reverse n) = UnitarySem.uc_eval (QPE.QFT_w_reverse n).
 Proof.
@@ -156,44 +223,279 @@ Proof.
   reflexivity.
 Qed.
 
-Lemma controlled_powers_var_same : forall n (f : nat -> bccom) k (f' : nat -> base_ucom n),
-  (* some precondition relating f and f' *)
-  uc_eval (k + n) (controlled_powers_var f k) = 
+Lemma QFT_w_reverse_WF : forall n, well_formed (QFT_w_reverse n).
+Proof. constructor. apply QFT_WF. apply reverse_qubits_WF. Qed.
+
+Lemma controlled_powers_same : forall n (f : nat -> bccom) k (f' : nat -> base_ucom n),
+  (k > 0)%nat ->
+  (forall i, uc_eval (k + n) (bc2ucom (f i)) = UnitarySem.uc_eval (cast (f' i) (k + n))) ->
+  (forall i j, (j < k)%nat -> is_fresh j (cast (f' i) (k + n))) ->
+  (forall i j, (j < k)%nat -> bcfresh j (f i)) ->
+  uc_eval (k + n) (controlled_powers f k) = 
     UnitarySem.uc_eval (QPE.controlled_powers_var f' k).
 Proof.
-  assert (H : forall n f k kmax f',
-    uc_eval (kmax + n) (bc2ucom (controlled_powers_var' f k kmax)) =
+  assert (H : forall n (f : nat -> bccom) (f' : nat -> base_ucom n) k kmax,
+    (kmax > 0)%nat ->
+    (forall i, uc_eval (kmax + n) (bc2ucom (f i)) = 
+          UnitarySem.uc_eval (cast (f' i) (kmax + n))) ->
+    (forall i j, (j < kmax)%nat -> is_fresh j (cast (f' i) (kmax + n))) ->
+    (forall i j, (j < kmax)%nat -> bcfresh j (f i)) ->
+    uc_eval (kmax + n) (bc2ucom (controlled_powers' f k kmax)) = 
       UnitarySem.uc_eval (@QPE.controlled_powers_var' n f' k kmax)).
-  { intros n f k kmax f'.
+  { intros n f f' k kmax Hkmax Hfeq Hfr' Hfr.
     destruct k; try reflexivity.
-    induction k.
-    unfold uc_eval; simpl.  
-    admit.
-    admit. }
-  intros.
-  apply H.
-Admitted.
+    induction k. 
+    simpl. 
+    rewrite control_correct.  
+    rewrite cast_control_commute.
+    apply control_cong.
+    apply Hfeq.
+    split; intro H.
+    apply Hfr'. lia.
+    apply bcfresh_is_fresh.
+    apply Hfr. lia.
+    apply bc2ucom_WF.
+    replace (controlled_powers' f (S (S k)) kmax)
+      with (bcseq (controlled_powers' f (S k) kmax)
+                  (bccont (kmax - (S k) - 1) (f (S k)))) 
+      by reflexivity.
+    replace (controlled_powers_var' f' (S (S k)) kmax)
+      with (controlled_powers_var' f' (S k) kmax ;
+            cast (UnitaryOps.control (kmax - (S k) - 1) (f' (S k))) (kmax + n))%ucom 
+      by reflexivity.
+    remember (S k) as k'.
+    unfold uc_eval in *.
+    simpl in *.
+    rewrite IHk.
+    apply f_equal2; try reflexivity.
+    specialize control_correct as aux.
+    unfold uc_eval in aux.
+    rewrite aux. clear aux.
+    rewrite cast_control_commute.
+    apply control_cong.
+    apply Hfeq.
+    split; intro H.
+    apply Hfr'. lia.
+    apply bcfresh_is_fresh.
+    apply Hfr. lia.
+    apply bc2ucom_WF. }
+  intros. apply H; auto.
+Qed.
 
-
-
-(* ... and so on, ending with QPE_var_same *)
-
-(* Final correctness property is a wrapper around Shor_correct_full_implementation
-   in Shor.v *)
-
-(*
-Lemma Shor_correct_full_implementation :
-  exists β, 
-    β>0 /\
-    forall (a N : nat),
-      (0 < a < N)%nat ->
-      (Nat.gcd a N = 1)%nat ->
-      let m := Nat.log2 (2 * N^2)%nat in
-      let n := Nat.log2 (2 * N)%nat in
-      probability_of_success_var a (ord a N) N m n (modmult_rev_anc n) (f_modmult_circuit a (modinv a N) N n) >= β / (Nat.log2 N)^4.
+Lemma map_bccom_eq_map_qubits : forall f bc,
+  bcelim bc <> bcskip ->
+  bc2ucom (map_bccom f (bcelim bc)) = map_qubits f (bc2ucom (bcelim bc)).
 Proof.
+  intros f bc H.
+  induction bc; simpl in *; try reflexivity.
+  contradict H; reflexivity.
+  destruct (bcelim bc). contradiction.
+  1-2: try rewrite IHbc by easy; reflexivity.
+  simpl bc2ucom.
+  rewrite map_qubits_control.
+  simpl in IHbc.
+  rewrite IHbc by easy.
+  reflexivity.
+  apply control'_WF.
+  apply bc2ucom_WF.
+  simpl bc2ucom.
+  rewrite map_qubits_control.
+  simpl in IHbc.
+  rewrite IHbc by easy.
+  reflexivity.
+  constructor; apply bc2ucom_WF.
+  destruct (bcelim bc1); destruct (bcelim bc2); try easy;
+    simpl in *; try rewrite IHbc2; try rewrite IHbc1; easy.
+Qed.
 
-(* Double check that we're not using admitted lemmas *)
-Print Assumptions shor_circuit_correct.
+Lemma map_qubits_bcfresh : forall k q (bc : bccom),
+  (q < k)%nat ->
+  bcelim bc <> bcskip ->
+  bcfresh q (map_bccom (fun i : nat => (k + i)%nat) (bcelim bc)).
+Proof.
+  intros k q bc Hq H.
+  induction bc. simpl. 
+  contradict H; reflexivity.
+  1-2: simpl; constructor; lia.
+  simpl. 
+  destruct (bcelim bc) eqn:bce.
+  contradict H.
+  simpl. rewrite bce. reflexivity.
+  1-4: simpl in *; constructor; try lia; apply IHbc; easy.
+  simpl.
+  destruct (bcelim bc1) eqn:bce1; destruct (bcelim bc2) eqn:bce2.
+  contradict H.
+  simpl. rewrite bce1, bce2. reflexivity.
+  all: try (apply IHbc1; easy).
+  all: try (apply IHbc2; easy).
+  all: simpl; constructor.
+  all: try (apply IHbc1; easy).
+  all: try (apply IHbc2; easy).
+Qed.
 
-*)
+Local Opaque npar controlled_powers QFT_w_reverse QPE.QFT_w_reverse.
+Lemma QPE_same : forall k n (f : nat -> bccom) (f' : nat -> base_ucom n),
+  (k > 0)%nat -> (n > 0)%nat ->
+  (forall i, bcelim (f i) <> bcskip) ->
+  (forall i, uc_eval n (bc2ucom (bcelim (f i))) = UnitarySem.uc_eval (f' i)) ->
+  uc_eval (k + n) (QPE k (fun i => bcelim (f i))) = 
+    UnitarySem.uc_eval (QPE.QPE_var k n f').
+Proof.
+  intros k n f f' Hk Hn Hf1 Hf2.
+  unfold uc_eval. simpl.
+  repeat apply f_equal2.
+  - specialize change_dim as H.
+    unfold uc_eval in H.
+    rewrite H with (n:=k). 
+    symmetry. apply cast_cong_r.
+    rewrite <- uc_well_typed_invert. 
+    apply QFT_w_reverse_WT.
+    assumption.
+    symmetry. 
+    specialize invert_same as aux.
+    unfold uc_eval in aux.
+    unfold uc_equiv.
+    rewrite aux. 
+    rewrite <- 2 invert_correct.
+    apply f_equal.
+    apply QFT_w_reverse_same.
+    apply QFT_w_reverse_WF.
+  - apply controlled_powers_same; auto.
+    intro i.
+    rewrite map_bccom_eq_map_qubits.
+    rewrite change_dim with (n:=n).
+    unfold uc_eval in *.
+    rewrite map_qubits_same.
+    apply cast_cong_l.
+    apply Hf2.
+    apply bc2ucom_WF.
+    apply Hf1.
+    intros i j Hj.
+    apply map_qubits_fresh; auto.
+    intros i j Hj.
+    apply map_qubits_bcfresh; auto.
+  - specialize change_dim as H.
+    unfold uc_eval in H.
+    rewrite H with (n:=k). 
+    symmetry. apply cast_cong_r. 
+    apply npar_WT.
+    assumption.
+    symmetry. apply npar_H_same.
+Qed.
+
+(* Compute the effect of running (shor_circuit a N) on the all-zero input state. *)
+Definition run_shor_circuit a N := 
+  let m := Nat.log2 (2 * N^2)%nat in
+  let n := Nat.log2 (2 * N) in
+  let numq := num_qubits n in
+  @Mmult _ _ 1 (uc_eval (m+numq) (shor_circuit a N))
+               (basis_vector (2^(m+numq)) 0).
+
+(* Returns the probability that (shor_circuit a N) outputs x. *)
+Definition prob_shor_outputs a N x := 
+  let m := Nat.log2 (2 * N^2)%nat in
+  let n := Nat.log2 (2 * N) in
+  let numq := num_qubits n in
+  @prob_partial_meas _ numq (basis_vector (2^m) x) (run_shor_circuit a N).
+
+Local Opaque genM0 modmult_full reverser bcinv.
+Lemma bcelim_modmult_rev_neq_bcskip : forall n M C Cinv,
+  bcelim (modmult_rev M C Cinv n) <> bcskip.
+Proof. 
+  intros.
+  unfold modmult_rev.
+  assert (bcelim (modmult M C Cinv (S (S n))) <> bcskip).
+  { unfold modmult.
+    assert (bcelim (swapperh1 (S (S n))) <> bcskip).
+    { unfold swapperh1.
+      simpl. 
+      destruct (bcelim (swapperh1' n (S (S n)))); easy. }
+    Local Opaque swapperh1.
+    simpl.
+    destruct (bcelim (swapperh1 (S (S n)))); 
+    destruct (bcelim (genM0 M (S (S n)))); 
+    destruct (bcelim (modmult_full C Cinv (S (S n))));
+    destruct (bcelim (bcinv (swapperh1 (S (S n)); genM0 M (S (S n)))%bccom));
+    easy. }
+  Local Opaque modmult.
+  simpl.
+  destruct (bcelim (bcinv (reverser n))); 
+  destruct (bcelim (modmult M C Cinv (S (S n))));
+  destruct (bcelim (reverser n));
+  easy.
+Qed.
+
+Lemma shor_circuit_same : forall a N x, 
+  (0 < N)%nat ->
+  let m := Nat.log2 (2 * N^2)%nat in
+  let n := Nat.log2 (2 * N)%nat in
+  let anc := modmult_rev_anc n in
+  let f := Shor.f_modmult_circuit a (modinv a N) N n in
+  prob_shor_outputs a N x = 
+    prob_partial_meas (basis_vector (2^m) x) (Shor.Shor_final_state_var m n anc f).
+Proof.
+  intros a N x H m n anc f.
+  unfold prob_shor_outputs, run_shor_circuit.
+  subst m n anc.
+  apply f_equal.
+  unfold uc_eval, num_qubits, shor_circuit, Shor.Shor_final_state_var.
+  Local Opaque Nat.mul Nat.pow QPE QPE.QPE_var.
+  simpl.
+  remember (Nat.log2 (2 * N ^ 2)) as m.
+  remember (Nat.log2 (2 * N)) as n.
+  assert (0 < n)%nat.
+  { subst. apply Nat.log2_pos. lia. }
+  assert (0 < m)%nat.
+  { subst. 
+    assert (1 <= N ^ 2)%nat.
+    rewrite <- (Nat.pow_1_l 2) at 1.
+    apply Nat.pow_le_mono_l. lia.
+    apply Nat.log2_pos. lia. }
+  clear Heqn Heqm.
+  rewrite Mmult_assoc.
+  apply f_equal2.
+  apply QPE_same; auto.
+  lia.
+  intro i.
+  apply bcelim_modmult_rev_neq_bcskip.
+  intro i.
+  subst f.
+  unfold f_modmult_circuit, modexp.
+  rewrite bc2ucom_correct.
+  rewrite bc2ucom_csplit.
+  reflexivity.
+  apply eWT_bcWT.
+  apply bcelim_modmult_rev_neq_bcskip.
+  apply modmult_rev_eWT; auto.
+  rewrite 4 basis_f_to_vec_alt.
+  rewrite f_to_vec_X by lia.
+  rewrite f_to_vec_merge.
+  restore_dims .
+  rewrite f_to_vec_merge.
+  rewrite Nat.add_assoc.
+  apply f_to_vec_eq; intros i Hi.
+  bdestruct (i <? m + n).
+  bdestruct (i <? m).
+  rewrite update_index_neq by lia.
+  rewrite 2 nat_to_funbool_0.
+  reflexivity.
+  bdestruct (i =? m + n - 1).
+  subst i.
+  rewrite update_index_eq.
+  rewrite nat_to_funbool_0, nat_to_funbool_1. 
+  bdestructΩ (m + n - 1 - m =? n - 1).
+  reflexivity.
+  rewrite update_index_neq by lia.
+  rewrite nat_to_funbool_0, nat_to_funbool_1. 
+  bdestructΩ (i - m =? n - 1).
+  reflexivity.
+  rewrite update_index_neq by lia.
+  rewrite 2 nat_to_funbool_0.
+  reflexivity.
+  apply pow_positive; lia.
+  apply Nat.pow_gt_1; lia.
+  apply pow_positive; lia.
+  apply pow_positive; lia.
+Qed.
+
+
